Removed syntax for subblock-opsem, symbolic execution works on the same syntax as ./ssa/ssa_def.ott, such that they can share the same well-formedness rules and other supporting lemmas, and we dont need to define translations between them. This simplifies the proof a lot.
To adopt this syntax, SE uses input with dependent properties that prove if inputs
are of insn_call (insn_call is the branching insn in subblock-opsem, but
a common insn in ssa-opsem). We also defined functions that generate such 'dependent' inputs from 'raw'
syntax, and translations in between. 



git-svn-id: https://webdav.seas.upenn.edu/svn/sol/vol@2538 eef5ea85-cc2e-0410-bd84-0fae1f012da8

src/TV/symexe_correct.v
@@ -20,19 +20,19 @@ Export SimpleSE.
 
 (* Correctness of the cmds validator *)
 
-Definition tv_cmds (cs1 cs2 : list cmd) (lc gl:GVMap) :=
-se_cmds (mkSstate (env_to_smap gl lc) smem_init sframe_init nil) cs1 =
-se_cmds (mkSstate (env_to_smap gl lc) smem_init sframe_init nil) cs2.
+Definition tv_cmds (nbs1 nbs2 : list nbranch) (lc gl:GVMap) :=
+se_cmds (mkSstate (env_to_smap gl lc) smem_init sframe_init nil) nbs1 =
+se_cmds (mkSstate (env_to_smap gl lc) smem_init sframe_init nil) nbs2.
 
-Lemma tv_cmds__is__correct : forall TD cs cs' lc1 als1 gl1 Mem1 lc2 als2 gl2 Mem2 tr,
+Lemma tv_cmds__is__correct : forall TD nbs nbs' lc1 als1 gl1 Mem1 lc2 als2 gl2 Mem2 tr,
   uniq gl1 ->
   uniq lc1 ->  
-  wf_cmds cs' ->
-  tv_cmds cs cs' lc1 gl1 ->
-  dbCmds TD lc1 als1 gl1 Mem1 cs lc2 als2 gl2 Mem2 tr ->
-  dbCmds TD lc1 als1 gl1 Mem1 cs' lc2 als2 gl2 Mem2 tr.
+  wf_nbranchs nbs' ->
+  tv_cmds nbs nbs' lc1 gl1 ->
+  dbCmds TD lc1 als1 gl1 Mem1 (nbranchs2cmds nbs) lc2 als2 gl2 Mem2 tr ->
+  dbCmds TD lc1 als1 gl1 Mem1 (nbranchs2cmds nbs') lc2 als2 gl2 Mem2 tr.
 Proof.
-  intros TD cs cs' lc1 als1 gl1 Mem1 lc2 als2 gl2 Mem2 tr Huniqg Huniqc Wf Htv_cmds HdbCmds.
+  intros TD nbs nbs' lc1 als1 gl1 Mem1 lc2 als2 gl2 Mem2 tr Huniqg Huniqc Wf Htv_cmds HdbCmds.
   unfold tv_cmds in Htv_cmds.
   assert (Uniqs:=HdbCmds).
   apply dbCmds_uniq in Uniqs; auto.
@@ -42,13 +42,20 @@ Proof.
   apply se_cmds__denote__op_cmds; auto.
 Qed.
 
+Record subblock := mkSB
+{
+  NBs : list nbranch;
+  call_cmd : cmd;
+  call_cmd_isCall : Instruction.isCallInst call_cmd = true
+}.
+
 Definition tv_subblock (sb1 sb2:subblock) (lc gl:GVMap) :=
 match (sb1, sb2) with
-| (subblock_intro cs1 call1, subblock_intro cs2 call2) =>
-  let st1 := se_cmds (mkSstate (env_to_smap gl lc) smem_init sframe_init nil) cs1 in
-  let st2 := se_cmds (mkSstate (env_to_smap gl lc) smem_init sframe_init nil) cs2 in
-  let cl1 := se_call st1 call1 in
-  let cl2 := se_call st2 call2 in
+| (mkSB nbs1 call1 iscall1, mkSB nbs2 call2 iscall2) =>
+  let st1 := se_cmds (mkSstate (env_to_smap gl lc) smem_init sframe_init nil) nbs1 in
+  let st2 := se_cmds (mkSstate (env_to_smap gl lc) smem_init sframe_init nil) nbs2 in
+  let cl1 := se_call st1 call1 iscall1 in
+  let cl2 := se_call st2 call2 iscall2 in
   st1 = st2 /\ call1 = call2
 end.
 
@@ -66,10 +73,35 @@ match (ps1, ps2) with
 | _ => False
 end.
 
+Fixpoint cmds2sbs (cs:list cmd) : (list subblock*list nbranch) :=
+match cs with
+| nil => (nil,nil)
+| c::cs' =>
+  match (isCallInst_dec c) with
+  | left isnotcall => 
+    match (cmds2sbs cs') with
+    | (nil, nbs0) => (nil, mkNB c isnotcall::nbs0) 
+    | (mkSB nbs call0 iscall0::sbs', nbs0) => 
+      (mkSB (mkNB c isnotcall::nbs) call0 iscall0::sbs', nbs0) 
+    end
+  | right iscall => 
+    match (cmds2sbs cs') with
+    | (sbs, nbs0) => (mkSB nil c iscall::sbs, nbs0) 
+    end
+  end
+end.
+
 Definition tv_block (b1 b2:block) (lc gl:GVMap) :=
 match (b1, b2) with
-| (block_intro l1 ps1 sbs1 tmn1, block_intro l2 ps2 sbs2 tmn2) =>
-  l1 = l2 /\ tv_phinodes ps1 ps2 /\ tv_subblocks sbs1 sbs2 lc gl /\ tmn1 = tmn2
+| (block_intro l1 ps1 cs1 tmn1, block_intro l2 ps2 cs2 tmn2) =>
+  match (cmds2sbs cs1, cmds2sbs cs2) with
+  | ((sbs1, nbs1), (sbs2, nbs2)) =>
+    l1 = l2 /\ 
+    tv_phinodes ps1 ps2 /\ 
+    tv_subblocks sbs1 sbs2 lc gl /\ 
+    tv_cmds nbs1 nbs2 lc gl /\ 
+    tmn1 = tmn2
+  end
 end.
 
 Fixpoint tv_blocks (bs1 bs2:list block) (lc gl:GVMap) :=
@@ -113,9 +145,9 @@ match (S1, S2) with
 end.
 
 Inductive wf_subblock : subblock -> Prop :=
-| wf_subblock_intro : forall cs call0, 
-  wf_cmds cs ->
-  wf_subblock (subblock_intro cs call0).
+| wf_subblock_intro : forall nbs call0 iscall0, 
+  wf_nbranchs nbs ->
+  wf_subblock (mkSB nbs call0 iscall0).
 
 Inductive wf_subblocks : list subblock -> Prop :=
 | wf_subblocks_nil : wf_subblocks nil
@@ -125,9 +157,11 @@ Inductive wf_subblocks : list subblock -> Prop :=
   wf_subblocks (sb::sbs).
 
 Inductive wf_block : block -> Prop :=
-| wf_block_intro : forall l ps sbs tmn, 
+| wf_block_intro : forall l ps cs sbs nbs tmn, 
+  cmds2sbs cs = (sbs,nbs) ->
   wf_subblocks sbs ->
-  wf_block (block_intro l ps sbs tmn).
+  wf_nbranchs nbs ->
+  wf_block (block_intro l ps cs tmn).
 
 Lemma tv_terminator__is__correct : forall TD fh1 lb1 fh2 lb2 B1 B2 lc gl tmn B1' lc' tr,
   tv_fdef (fdef_intro fh1 lb1) (fdef_intro fh2 lb2) gl0 ->
@@ -170,26 +204,30 @@ Definition tv_dbCall__is__correct_prop S1 TD Ps1 lc gl Mem0 call0 lc' gl' Mem' t
   tv_system S1 S2 ->
   tv_products Ps1 Ps2 ->
   dbCall S2 TD Ps2 lc gl Mem0 call0 lc' gl' Mem' tr.
-Definition tv_subblock__is__correct_prop S1 TD Ps1 lc als gl Mem sb1 lc' als' gl' Mem' tr
-  (db:dbSubblock S1 TD Ps1 lc als gl Mem sb1 lc' als' gl' Mem' tr) :=
-  forall S2 Ps2 sb2,
+Definition tv_subblock__is__correct_prop S1 TD Ps1 lc als gl Mem cs1 lc' als' gl' Mem' tr
+  (db:dbSubblock S1 TD Ps1 lc als gl Mem cs1 lc' als' gl' Mem' tr) :=
+  forall S2 Ps2 cs2 sb1 sb2,
   uniq gl ->
   uniq lc ->
+  cmds2sbs cs1 = (sb1::nil, nil) ->
+  cmds2sbs cs2 = (sb2::nil, nil) ->
   wf_subblock sb2 ->
   tv_system S1 S2 ->
   tv_products Ps1 Ps2 ->
   tv_subblock sb1 sb2 lc gl ->
-  dbSubblock S2 TD Ps2 lc als gl Mem sb2 lc' als' gl' Mem' tr.
-Definition tv_subblocks__is__correct_prop S1 TD Ps1 lc als gl Mem sbs1 lc' als' gl' Mem' tr
-  (db:dbSubblocks S1 TD Ps1 lc als gl Mem sbs1 lc' als' gl' Mem' tr) :=
-  forall S2 Ps2 sbs2,
+  dbSubblock S2 TD Ps2 lc als gl Mem cs2 lc' als' gl' Mem' tr.
+Definition tv_subblocks__is__correct_prop S1 TD Ps1 lc als gl Mem cs1 lc' als' gl' Mem' tr
+  (db:dbSubblocks S1 TD Ps1 lc als gl Mem cs1 lc' als' gl' Mem' tr) :=
+  forall S2 Ps2 sbs1 sbs2 cs2,
   uniq gl ->
   uniq lc ->
+  cmds2sbs cs1 = (sbs1, nil) ->
+  cmds2sbs cs2 = (sbs2, nil) ->
   wf_subblocks sbs2 ->
   tv_system S1 S2 ->
   tv_products Ps1 Ps2 ->
   tv_subblocks sbs1 sbs2 lc gl ->
-  dbSubblocks S2 TD Ps2 lc als gl Mem sbs2 lc' als' gl' Mem' tr.
+  dbSubblocks S2 TD Ps2 lc als gl Mem cs2 lc' als' gl' Mem' tr.
 Definition tv_block__is__correct_prop S1 TD Ps1 F1 arg state1 state2 tr
   (db:dbBlock S1 TD Ps1 F1 arg state1 state2 tr) :=
   forall S2 Ps2 fh1 lb1 fh2 lb2 B1 lc als gl Mem B1' lc' als' gl' Mem' B2,
@@ -214,26 +252,26 @@ Definition tv_block__is__correct_prop S1 TD Ps1 F1 arg state1 state2 tr
 Definition tv_blocks__is__correct_prop S1 TD Ps1 F1 lp state1 state2 tr
   (db:dbBlocks S1 TD Ps1 F1 lp state1 state2 tr) :=
   forall S2 Ps2 fh1 lb1 fh2 lb2 gl lc n tmn1
-                            l1 ps1 sbs1 ps1' l1' als
-                            lc' gl' Mem Mem' als' tmn1' sbs1',
-  state1 = (mkState (mkEC (block_intro l1 ps1 sbs1 tmn1) lc als) gl Mem) ->
-  state2 = (mkState (mkEC (block_intro l1' ps1' sbs1' tmn1') lc' als') gl' Mem') ->
+                            l1 ps1 cs1 ps1' l1' als
+                            lc' gl' Mem Mem' als' tmn1' cs1',
+  state1 = (mkState (mkEC (block_intro l1 ps1 cs1 tmn1) lc als) gl Mem) ->
+  state2 = (mkState (mkEC (block_intro l1' ps1' cs1' tmn1') lc' als') gl' Mem') ->
   tv_system S1 S2 ->
   tv_products Ps1 Ps2 ->
   F1 = fdef_intro fh1 lb1 ->
   tv_fdef (fdef_intro fh1 lb1) (fdef_intro fh2 lb2) gl0 ->
   tv_blocks lb1 lb2 lc gl ->
-  nth_error lb1 n = Some (block_intro l1 ps1 sbs1 tmn1) ->
-  exists l2, exists ps2, exists sbs2, exists tmn2, 
-  exists l2', exists ps2', exists sbs2', exists tmn2', exists n',
-    nth_error lb2 n = Some (block_intro l2 ps2 sbs2 tmn2) /\
-    nth_error lb1 n' = Some (block_intro l1' ps1' sbs1' tmn1') /\
-    nth_error lb2 n' = Some (block_intro l2' ps2' sbs2' tmn2') /\
-    tv_block (block_intro l1 ps1 sbs1 tmn1) (block_intro l2 ps2 sbs2 tmn2) lc gl /\
-    tv_block (block_intro l1' ps1' sbs1' tmn1') (block_intro l2' ps2' sbs2' tmn2') lc gl /\
+  nth_error lb1 n = Some (block_intro l1 ps1 cs1 tmn1) ->
+  exists l2, exists ps2, exists cs2, exists tmn2, 
+  exists l2', exists ps2', exists cs2', exists tmn2', exists n',
+    nth_error lb2 n = Some (block_intro l2 ps2 cs2 tmn2) /\
+    nth_error lb1 n' = Some (block_intro l1' ps1' cs1' tmn1') /\
+    nth_error lb2 n' = Some (block_intro l2' ps2' cs2' tmn2') /\
+    tv_block (block_intro l1 ps1 cs1 tmn1) (block_intro l2 ps2 cs2 tmn2) lc gl /\
+    tv_block (block_intro l1' ps1' cs1' tmn1') (block_intro l2' ps2' cs2' tmn2') lc gl /\
     dbBlocks S2 TD Ps2 (fdef_intro fh2 lb2) lp
-      (mkState (mkEC (block_intro l2 ps2 sbs2 tmn2) lc als) gl Mem)
-      (mkState (mkEC (block_intro l2' ps2' sbs2' tmn2') lc' als') gl' Mem')
+      (mkState (mkEC (block_intro l2 ps2 cs2 tmn2) lc als) gl Mem)
+      (mkState (mkEC (block_intro l2' ps2' cs2' tmn2') lc' als') gl' Mem')
       tr.
 Definition tv_fdef__is__correct_prop fid rt lp S1 TD Ps1 lc gl Mem lc' gl' als' Mem' Rid oResult tr
   (db:dbFdef fid rt lp S1 TD Ps1 lc gl Mem lc' gl' als' Mem' Rid oResult tr) :=
@@ -252,6 +290,354 @@ Lemma tv_blocks_nth_Some_inv : forall lb1 lb2 lc gl n B1,
   exists B2, 
     nth_error lb2 n = Some B2 /\ tv_block B1 B2 lc gl.
 Admitted. (*nth*)
+
+Lemma cmds2sbs_nil_inv : forall cs,
+  cmds2sbs cs = (nil, nil) ->
+  cs = nil.
+Proof.
+  destruct cs; intros; auto.
+    simpl in H.
+    destruct (isCallInst_dec c).
+      destruct (cmds2sbs cs).
+      destruct l0.
+        inversion H.
+        destruct s. inversion H.
+      destruct (cmds2sbs cs).
+      inversion H.
+Qed.
+
+Lemma cmds2sb_inv : forall cs sb,
+  cmds2sbs cs = (sb::nil, nil) ->
+  exists cs', exists call0,
+    cs = cs'++call0::nil /\
+    cmds2sbs cs' = (nil, NBs sb) /\
+    call_cmd sb = call0.
+Proof.
+  induction cs; intros; simpl in *.
+    inversion H.
+
+    remember (cmds2sbs cs) as R.
+    remember (isCallInst_dec a) as R'.
+    destruct R'.
+      destruct R.
+      destruct l0.
+        inversion H.
+
+        destruct s. inversion H; subst. clear H.
+        destruct (@IHcs (mkSB NBs0 call_cmd0 call_cmd_isCall0)) as [cs' [call0 [J1 [J2 J3]]]]; subst; auto.
+        clear IHcs.
+        simpl in *.
+        exists (a::cs').
+        exists (call_cmd0).
+        split; auto.
+        split; auto.
+          simpl.
+          rewrite J2.
+          rewrite <- HeqR'. auto.
+
+      destruct R.
+      inversion H; subst. clear H.
+      symmetry in HeqR.
+      apply cmds2sbs_nil_inv in HeqR. subst.
+      exists nil. exists a.
+      split; auto.
+Qed.
+
+Definition dbCmds__cmds2nbs : forall TD lc als gl Mem1 cs lc' als' gl' Mem2 tr, 
+  dbCmds TD lc als gl Mem1 cs lc' als' gl' Mem2 tr ->
+  exists nbs, cmds2sbs cs = (nil, nbs).
+Proof.
+  intros.
+  induction H; simpl.
+    exists nil. auto.
+
+    destruct IHdbCmds as [nbs J].
+    destruct (isCallInst_dec c).
+      rewrite J. exists (mkNB c e::nbs). auto.
+
+      apply dbCmd_isNotCallInst in H.
+      rewrite e in H. inversion H.
+Qed.
+
+Lemma dbCall_isCallInst : forall S TD Ps lc gl Mem1 c lc' gl' Mem2 tr,
+  dbCall S TD Ps lc gl Mem1 c lc' gl' Mem2 tr ->
+  Instruction.isCallInst c = true.
+Proof.
+  intros S TD Ps lc gl Mem1 c lc' gl' Mem2 tr HdbCall.
+  induction HdbCall; auto.
+Qed.
+
+Lemma cmdscall2sbs : forall cs call0 nbs
+  (isCall0:Instruction.isCallInst call0=true),
+  cmds2sbs cs = (nil, nbs) ->
+  isCallInst_dec call0 = right isCall0 ->
+  cmds2sbs (cs++call0::nil) = (mkSB nbs call0 isCall0::nil, nil).
+Proof.
+  induction cs; intros; simpl in *.
+    inversion H; subst.
+    rewrite H0. auto.
+
+    destruct (isCallInst_dec a).
+      remember (cmds2sbs cs) as R.
+      destruct R.
+      destruct l0.
+        inversion H; subst. clear H.
+        apply IHcs with (nbs:=l1) in H0; auto.
+        rewrite H0; auto.
+     
+        destruct s. inversion H.
+
+      destruct (cmds2sbs cs).
+      inversion H.
+Qed.
+
+Lemma dbSubblock__cmds2sb : forall S TD Ps lc1 als1 gl1 Mem1 cs lc2 als2 gl2 Mem2 tr,
+  dbSubblock S TD Ps lc1 als1 gl1 Mem1 cs lc2 als2 gl2 Mem2 tr ->
+  exists sb, cmds2sbs cs = (sb::nil, nil).
+Proof.
+  intros.
+  inversion H; subst.
+  apply dbCmds__cmds2nbs in H0.
+  destruct H0 as [nbs H0].
+  remember (isCallInst_dec call0) as R.
+  destruct R.
+    apply dbCall_isCallInst in H1.
+    rewrite e in H1. inversion H1.
+
+    exists (mkSB nbs call0 e).
+    apply cmdscall2sbs; auto.
+Qed.
+
+Lemma cmds_cons2sbs : forall cs cs' sb sbs',
+  cmds2sbs cs = (sb::nil, nil) ->
+  cmds2sbs cs' = (sbs', nil) ->
+  cmds2sbs (cs++cs') = (sb::sbs', nil).
+Proof.
+  induction cs; intros; simpl.
+    simpl in H. inversion H.
+
+    simpl in H.
+    destruct (isCallInst_dec a).
+      remember (cmds2sbs cs) as R.
+      destruct R.
+        destruct l0.
+          inversion H.
+
+          destruct s. inversion H; subst. clear H.
+          apply IHcs with (sb:=mkSB NBs0 call_cmd0 call_cmd_isCall0) in H0; auto.
+          clear IHcs.
+          rewrite H0. auto.
+ 
+      remember (cmds2sbs cs) as R.
+      destruct R.
+      inversion H; subst. clear H.
+      symmetry in HeqR.
+      apply cmds2sbs_nil_inv in HeqR. subst.
+      simpl.
+      rewrite H0. auto.
+Qed.
+
+Lemma dbSubblocks__cmds2sbs : forall S TD Ps lc1 als1 gl1 Mem1 cs lc2 als2 gl2 Mem2 tr,
+  dbSubblocks S TD Ps lc1 als1 gl1 Mem1 cs lc2 als2 gl2 Mem2 tr ->
+  exists sbs, cmds2sbs cs = (sbs, nil).
+Proof.
+  intros.
+  induction H; simpl.
+    exists nil. auto.
+
+    apply dbSubblock__cmds2sb in H.
+    destruct H as [sb H].
+    destruct IHdbSubblocks as [sbs H1].
+    exists (sb::sbs).
+    apply cmds_cons2sbs; auto.
+Qed.
+
+Lemma cmds_cons2sbs_inv : forall cs cs' sbs0 sb sbs',
+  cmds2sbs (cs++cs') = (sbs0, nil) ->
+  cmds2sbs cs = (sb::nil, nil) ->
+  cmds2sbs cs' = (sbs', nil) ->
+  sbs0 = sb::sbs'.
+Proof.
+  intros.
+  apply cmds_cons2sbs with (cs':=cs')(sbs':=sbs') in H0; auto.
+  rewrite H in H0.
+  inversion H0; auto.
+Qed.
+
+Lemma cmds2sbs_cons_inv : forall cs0 sb sbs',
+  cmds2sbs cs0 = (sb::sbs', nil) ->
+  exists cs, exists cs',
+    cmds2sbs cs = (sb::nil, nil) /\
+    cmds2sbs cs' = (sbs', nil) /\
+    cs0 = cs++cs'.
+Proof.
+  induction cs0; intros.
+    simpl in H. inversion H.
+
+    simpl in H.
+    remember (isCallInst_dec a) as R.
+    remember (cmds2sbs cs0) as R'.
+    destruct R.
+      destruct R'.
+        destruct l0.
+          inversion H.
+
+          destruct s. inversion H; subst. clear H.
+          destruct (@IHcs0 (mkSB NBs0 call_cmd0 call_cmd_isCall0) sbs') as [cs [cs' [J1 [J2 J3]]]]; subst; auto.
+          exists (a::cs). exists cs'.
+          split; auto.
+            simpl.
+            rewrite <- HeqR.
+            rewrite J1. auto.
+
+      destruct R'.
+      inversion H; subst. clear H.
+      destruct sbs'.
+        symmetry in HeqR'.
+        apply cmds2sbs_nil_inv in HeqR'. subst.
+        exists (a::nil). exists nil.
+        simpl. rewrite <- HeqR. auto.
+
+        destruct (@IHcs0 s sbs') as [cs [cs' [J1 [J2 J3]]]]; subst; auto.
+        exists (a::nil). exists (cs++cs').
+        simpl. rewrite <- HeqR. auto.
+Qed.
+
+Lemma cmds_rcons2sbs : forall cs cs' sbs nbs,
+  cmds2sbs cs = (sbs, nil) ->
+  cmds2sbs cs' = (nil, nbs) ->
+  cmds2sbs (cs++cs') = (sbs, nbs).
+Proof.
+  induction cs; intros.
+    simpl in H. inversion H; subst. auto.
+
+    simpl in *.
+    remember (cmds2sbs cs) as R.
+    destruct (isCallInst_dec a).
+      destruct R.
+        destruct l0.
+          inversion H.
+
+          destruct s. inversion H; subst. clear H.
+          apply IHcs with (sbs:=mkSB NBs0 call_cmd0 call_cmd_isCall0::l0) in H0; auto.
+          rewrite H0. auto.
+
+      destruct R.
+      inversion H; subst. clear H.
+      apply IHcs with (sbs:=l0) in H0; auto.
+      rewrite H0. auto.
+Qed.
+
+Lemma cmds_rcons2sbs_inv : forall cs cs' sbs0 nbs0 sbs nbs,
+  cmds2sbs (cs++cs') = (sbs0, nbs0) ->
+  cmds2sbs cs = (sbs, nil) ->
+  cmds2sbs cs' = (nil, nbs) ->
+  sbs0 = sbs /\ nbs0 = nbs.
+Proof.
+  intros.
+  apply cmds_rcons2sbs with (cs':=cs')(nbs:=nbs) in H0; auto.
+  rewrite H in H0. inversion H0; auto.
+Qed.
+ 
+Lemma cmds2nbranchs__cmds2nbs : forall cs nbs,
+  cmds2nbranchs cs = Some nbs ->
+  cmds2sbs cs = (nil, nbs).
+Proof.
+  induction cs; intros.
+    simpl in H. inversion H; auto.
+
+    simpl in *.
+    unfold cmd2nbranch in H.
+    destruct (isCallInst_dec a).
+      destruct (cmds2sbs cs).
+        remember (cmds2nbranchs cs) as R.
+        destruct R.
+          inversion H; subst. clear H.
+          assert (ret l2 = ret l2) as EQ. auto.
+          apply IHcs in EQ.
+          inversion EQ; subst. auto.
+
+          inversion H.
+      inversion H.
+Qed.
+
+Lemma cmds2nbs__nbranchs2cmds : forall nbs cs,
+  cmds2sbs cs = (nil, nbs) ->
+  nbranchs2cmds nbs = cs.
+Proof.
+  induction nbs; intros.
+    apply cmds2sbs_nil_inv in H. subst. auto.
+
+    simpl.
+    destruct a.
+    destruct cs.
+      simpl in H. inversion H.
+
+      simpl in H.
+      destruct (isCallInst_dec c).
+        remember (cmds2sbs cs) as R.
+        destruct R.
+        destruct l0.
+          inversion H; subst.
+          rewrite IHnbs with (cs:=cs); auto.
+
+          destruct s.
+          inversion H; subst.
+
+        destruct (cmds2sbs cs).
+        inversion H.
+Qed.
+
+
+Lemma cmds2nbranchs__nbranchs2cmds : forall cs nbs,
+  cmds2nbranchs cs = Some nbs ->
+  nbranchs2cmds nbs = cs.
+Proof.
+  intros.
+  apply cmds2nbs__nbranchs2cmds.
+  apply cmds2nbranchs__cmds2nbs; auto.
+Qed.
+
+Lemma cmds2sbs_inv : forall cs sbs nbs,
+  cmds2sbs cs = (sbs, nbs) ->
+  exists cs1, exists cs2, 
+    cs = cs1++cs2 /\
+    cmds2sbs cs1 = (sbs, nil) /\
+    cmds2sbs cs2 = (nil, nbs).
+Proof.
+  induction cs; intros.
+    simpl in H. inversion H; subst.
+    exists nil. exists nil. auto.
+
+    simpl in H.
+    remember (isCallInst_dec a) as R.
+    remember (cmds2sbs cs) as R'.
+    destruct R.
+      destruct R'.
+        destruct l0.
+          inversion H; subst. clear H.
+          
+          destruct (@IHcs nil l1) as [cs1 [cs2 [J1 [J2 J3]]]]; subst; auto.
+          apply cmds2sbs_nil_inv in J2. subst.
+          exists nil. exists (a::cs2).
+          simpl. rewrite <- HeqR. 
+          simpl in HeqR'. rewrite <- HeqR'.
+          split; auto.
+
+       destruct s.
+       inversion H; subst. clear H.
+       destruct (@IHcs (mkSB NBs0 call_cmd0 call_cmd_isCall0::l0) nbs) as [cs1 [cs2 [J1 [J2 J3]]]]; subst; auto.
+       clear IHcs.
+       exists (a::cs1). exists cs2.
+       simpl. rewrite <- HeqR. rewrite J2. auto.
+    
+     destruct R'.
+     inversion H; subst. clear H.
+     destruct (@IHcs l0 nbs) as [cs1 [cs2 [J1 [J2 J3]]]]; subst; auto.
+     clear IHcs.
+     exists (a::cs1). exists cs2.
+     simpl. rewrite <- HeqR. rewrite J2. auto.
+Qed.
 
 Lemma tv__is__correct :
   (forall S1 TD Ps1 lc gl Mem0 call0 lc' gl' Mem' tr db, 
@@ -292,38 +678,92 @@ Case "dbCall_intro".
     eauto.
 
 Case "dbSubblock_intro".
+  unfold tv_subblock in H7.
+  destruct sb1.
   destruct sb2.
-  unfold tv_subblock in H5.
-  simpl in H5.
-  destruct H5 as [EQ1 EQ2]; subst.
-  inversion H2; subst.
-  apply tv_cmds__is__correct with (cs':=l0) in d; eauto.
+  apply cmds2sb_inv in H2.
+  destruct H2 as [cs' [call1 [J1 [J2 J3]]]].
+  apply cmds2nbs__nbranchs2cmds in J2.
+  apply app_inj_tail in J1.
+  destruct J1; subst.
+  apply cmds2sb_inv in H3.
+  destruct H3 as [cs2' [call0 [J1 [J2 J3]]]]; subst.
+  apply cmds2nbs__nbranchs2cmds in J2.
+  destruct H7 as [EQ1 EQ2]; subst.
+  inversion H4; subst.
+  apply tv_cmds__is__correct with (nbs':=NBs1) in d; eauto.
 
 Case "dbSubblocks_nil".
-  destruct sbs2;try solve [auto | simpl in H4; inversion H4].
-  
+  simpl in H1. inversion H1; subst.
+  destruct sbs2;try solve [auto | simpl in H6; inversion H6].
+    apply cmds2sbs_nil_inv in H2; subst; auto.
+
 Case "dbSubblocks_cons".
-  destruct sbs2; simpl in H6; inversion H6.
-  clear H6.
-  inversion H3; subst. clear H3.  
-  apply H with (S2:=S2)(Ps2:=Ps2) in H7; auto.
+  assert (Hcs2sb := d).
+  apply dbSubblock__cmds2sb in Hcs2sb.
+  destruct Hcs2sb as [sb Hcs2sb].
+  assert (Hcs'2sbs := d0).
+  apply dbSubblocks__cmds2sbs in Hcs'2sbs.
+  destruct Hcs'2sbs as [sbs Hcs'2sbs].
+  apply cmds_cons2sbs_inv with (sb:=sb)(sbs':=sbs) in H3; auto.
+  subst.
+  simpl in H8.
+  destruct sbs2 ; simpl in H8; inversion H8.
+  clear H8.
+  apply cmds2sbs_cons_inv in H4.
+  destruct H4 as [cs21 [cs22 [cs212s [cs222sbs2 EQ]]]]; subst.
+  inversion H5; subst. clear H5.  
+  apply H with (S2:=S2)(Ps2:=Ps2)(cs2:=cs21) in H3; auto.
   assert (tv_subblocks sbs sbs2 lc2 gl2) as J. 
     admit. (*tv inclusion*)
-  apply H0 with (S2:=S2)(Ps2:=Ps2) in J; eauto.
-    admit. (*uniq*)
-    admit. (*uniq*)
+  assert (uniq lc2) as Uniqc2. admit. (*uniq*)
+  assert (uniq gl2) as Uniqg2. admit. (*uniq*)
+  apply H0 with (S2:=S2)(Ps2:=Ps2)(cs2:=cs22) in J; eauto.
 
 Case "dbBlock_intro".
   inversion H0; subst. clear H0.
   inversion H1; subst. clear H1.
-  destruct B2 as [l2 ps2 sbs2 tmn2].
+  destruct B2 as [l2 ps2 cs2 tmn2].
   unfold tv_block in H9.
-  destruct H9 as [EQ1 [Htv_phinodes [Htv_subblocks EQ2]]]; subst.
+  remember (cmds2sbs (cs++cs')) as R1.
+  remember (cmds2sbs cs2) as R2.
+  destruct R1 as [sbs1 nbs1].
+  destruct R2 as [sbs2 nbs2].
+  destruct H9 as [EQ1 [Htv_phinodes [Htv_subblocks [Htv_cmds EQ2]]]]; subst.
+
+  assert (Hcs2sbs1 := d).
+  apply dbSubblocks__cmds2sbs in Hcs2sbs1.
+  destruct Hcs2sbs1 as [sbs Hcs2sbs1].
+  assert (Hcs2nbs1 := d0).
+  apply dbCmds__cmds2nbs in Hcs2nbs1.
+  destruct Hcs2nbs1 as [nbs Hcs2nbs1].
+ 
+  assert (J:=HeqR1).
+  symmetry in J.
+  apply cmds_rcons2sbs_inv with (sbs:=sbs)(nbs:=nbs) in J; auto using cmds2nbranchs__cmds2nbs.
+  destruct J; subst.
+
+  assert (J:=HeqR2).
+  symmetry in J.
+  apply cmds2sbs_inv in J.
+  destruct J as [cs1 [cs3 [EQ [Hcs12sbs2 Hcs32nbs2]]]]; subst.
   inversion H5; subst. clear H5.
+
+  apply cmds_rcons2sbs_inv with (sbs:=sbs2)(nbs:=nbs2) in H9; auto.
+  destruct H9; subst.
   assert (J:=Htv_subblocks).
-  apply H with (S2:=S2)(Ps2:=Ps2) in J; auto.
-  apply tv_terminator__is__correct with (B2:=block_intro l2 ps2 sbs2 tmn2)(fh2:=fh2)(lb2:=lb2) in d0; auto.
-    destruct d0 as [B2' [n [Htv_block1'2' [J2 [J3 Hdb]]]]].
+  apply H with (S2:=S2)(Ps2:=Ps2)(cs2:=cs1) in J; auto.
+  clear H.
+
+  apply cmds2nbs__nbranchs2cmds in Hcs2nbs1. subst.
+  apply cmds2nbs__nbranchs2cmds in Hcs32nbs2. subst.
+  assert (tv_cmds nbs nbs2 lc2 gl2) as Htv_cmds'.
+    admit. (*tv inclusion*)
+  assert (uniq lc2) as Uniqc2. admit.
+  assert (uniq gl2) as Uniqg2. admit.
+  apply tv_cmds__is__correct with (nbs':=nbs2) in d0; auto.
+  apply tv_terminator__is__correct with (B2:=block_intro l2 ps2 (cs1++nbranchs2cmds nbs2) tmn2)(fh2:=fh2)(lb2:=lb2) in d1; auto.
+    destruct d1 as [B2' [n [Htv_block1'2' [J2 [J3 Hdb]]]]].
     exists B2'. exists n. 
     split; eauto.
     split; auto.
@@ -332,40 +772,45 @@ Case "dbBlock_intro".
       admit. (*tv inclusion*)
 
     unfold tv_block.
+    rewrite <- HeqR1.
+    rewrite <- HeqR2.
     split; auto.
     split; auto.
-    split; auto.
+    split.
       clear - Htv_subblocks.
+      admit. (*tv inclusion*)      
+    split; auto.
+      clear - Htv_cmds.
       admit. (*tv inclusion*)      
 
 Case "dbBlocks_nil".
   inversion H0; subst. clear H0.
-  apply tv_blocks_nth_Some_inv with (n:=n)(B1:=block_intro l1' ps1' sbs1' tmn1') in H5; auto.
-  destruct H5 as [[l2 ps2 sbs2 tmn2] [Hnth_error2 Htv_block]].
-  exists l2. exists ps2. exists sbs2. exists tmn2.
-  exists l2. exists ps2. exists sbs2. exists tmn2. 
+  apply tv_blocks_nth_Some_inv with (n:=n)(B1:=block_intro l1' ps1' cs1' tmn1') in H5; auto.
+  destruct H5 as [[l2 ps2 cs2 tmn2] [Hnth_error2 Htv_block]].
+  exists l2. exists ps2. exists cs2. exists tmn2.
+  exists l2. exists ps2. exists cs2. exists tmn2. 
   exists n.
   split; auto.
 
 Case "dbBlocks_cons".
   inversion d; subst.
   assert (J:=H7).  
-  apply tv_blocks_nth_Some_inv with (n:=n)(B1:=block_intro l1 ps1 sbs1 tmn1) in J; auto.
-  destruct J as [[l2 ps2 sbs2 tmn2] [Hnth_error2 Htv_block12]].
+  apply tv_blocks_nth_Some_inv with (n:=n)(B1:=block_intro l1 ps1 (cs++cs') tmn1) in J; auto.
+  destruct J as [[l2 ps2 cs2 tmn2] [Hnth_error2 Htv_block12]].
   assert (J:=Htv_block12).
-  apply H with (S2:=S0)(Ps2:=Ps2)(fh3:=fh2)(lb3:=lb2)(fh2:=fh1)(lb2:=lb1)(Mem:=Mem0)(B1':=B')(lc':=lc3)(als':=als2)(gl':=gl2)(Mem':=Mem2)(als0:=als) in J; auto.
+  apply H with (S2:=S0)(Ps2:=Ps2)(fh3:=fh2)(lb3:=lb2)(fh2:=fh1)(lb2:=lb1)(Mem:=Mem0)(B1':=B')(lc':=lc4)(als':=als3)(gl':=gl3)(Mem':=Mem3)(als0:=als) in J; auto.
     destruct J as [B2' [n' [Hdb [J1 [J2 Htv_block12']]]]].
     clear H.
-    destruct B' as [l3 ps3 sbs3 tmn3].
-    assert (tv_blocks lb1 lb2 lc3 gl2) as H.
+    destruct B' as [l3 ps3 cs3 tmn3].
+    assert (tv_blocks lb1 lb2 lc4 gl3) as H.
       admit. (*tv inclusion*)      
     apply H0 with (S2:=S0)(Ps2:=Ps2)(fh2:=fh1)(fh3:=fh2)(n:=n')(tmn1:=tmn3)
-      (l1:=l3)(ps1:=ps3)(sbs1:=sbs3)(ps1'0:=ps1')(l1'0:=l1')(als:=als2)(lc'0:=lc')(gl'0:=gl')
-      (Mem:=Mem2)(Mem'0:=Mem')(als'0:=als')(tmn1'0:=tmn1')(sbs1'0:=sbs1') in H; auto.
-    destruct H as [l4 [ps4 [sbs4 [tmn4 [l4' [ps4' [sbs4' [tmn4' [n'' [J3 [J4 [J5 [J6 [J7 J8]]]]]]]]]]]]]].
+      (l1:=l3)(ps1:=ps3)(cs1:=cs3)(ps1'0:=ps1')(l1'0:=l1')(als:=als3)(lc'0:=lc')(gl'0:=gl')
+      (Mem:=Mem3)(Mem'0:=Mem')(als'0:=als')(tmn1'0:=tmn1')(cs1'0:=cs1') in H; auto.
+    destruct H as [l4 [ps4 [cs4 [tmn4 [l4' [ps4' [cs4' [tmn4' [n'' [J3 [J4 [J5 [J6 [J7 J8]]]]]]]]]]]]]].
     clear H0.
-    exists l2. exists ps2. exists sbs2. exists tmn2.
-    exists l4'. exists ps4'. exists sbs4'. exists tmn4'.
+    exists l2. exists ps2. exists cs2. exists tmn2.
+    exists l4'. exists ps4'. exists cs4'. exists tmn4'.
     exists n''.
     split; auto.
     split; auto.
@@ -396,33 +841,66 @@ Case "dbFdef_func".
       admit. (*tv inclusion*)      
     apply H with (S2:=S2)(Ps2:=Ps2)(fh1:=fheader_intro rt fid la)(fh2:=fheader_intro rt fid la)(n:=0)
       (ps1':=ps2)(l1':=l2)(als:=nil)(lc':=lc1)(gl':=gl1)
-      (Mem:=Mem0)(Mem':=Mem1)(als':=als1)(tmn1':=insn_return rid rt Result)(sbs1':=sbs2) 
-      (ps3:=ps1)(sbs3:=sbs1)(tmn2:=tmn1)(l3:=l1)in Htv_blocks; auto.
+      (Mem:=Mem0)(Mem':=Mem1)(als':=als1)(tmn1':=insn_return rid rt Result)(cs1':=cs21++cs22) 
+      (ps3:=ps1)(cs2:=cs1)(tmn2:=tmn1)(l3:=l1)in Htv_blocks; auto.
       clear H.
-      destruct Htv_blocks as [l3 [ps3 [sbs3 [tmn2 [l2' [ps2' [sbs2' [tmn2' [n' [J1 [J2 [J3 [J4 [J5 J6]]]]]]]]]]]]]].
+      destruct Htv_blocks as [l3 [ps3 [cs3 [tmn2 [l2' [ps2' [cs2' [tmn2' [n' [J1 [J2 [J3 [J4 [J5 J6]]]]]]]]]]]]]].
 
       unfold tv_block in J5.
-      destruct J5 as [EQ [Htv_phinodes [Htv_subblocks EQ']]]; subst.
-      assert (tv_subblocks sbs2 sbs2' lc1 gl1) as Htv_subblocks'.
+
+      remember (cmds2sbs (cs21++cs22)) as R1.
+      remember (cmds2sbs cs2') as R2.
+      destruct R1 as [sbs1 nbs1].
+      destruct R2 as [sbs2 nbs2].
+      destruct J5 as [EQ1 [Htv_phinodes [Htv_subblocks [Htv_cmds EQ2]]]]; subst.
+
+      assert (Hcs21sbs1 := d0).
+      apply dbSubblocks__cmds2sbs in Hcs21sbs1.
+      destruct Hcs21sbs1 as [sbs Hcs21sbs1].
+      assert (Hcs22nbs1 := d1).
+      apply dbCmds2nbranchs in Hcs22nbs1.
+      destruct Hcs22nbs1 as [nbs Hcs22nbs1].
+
+      assert (J:=HeqR1).
+      symmetry in J.
+      apply cmds_rcons2sbs_inv with (sbs:=sbs)(nbs:=nbs) in J; auto using cmds2nbranchs__cmds2nbs.
+      destruct J; subst.
+
+      assert (J:=HeqR2).
+      symmetry in J.
+      apply cmds2sbs_inv in J.
+      destruct J as [cs41 [cs42 [EQ [Hcs41sbs2 Hcs42nbs2]]]]; subst.
+
+      assert (J:=HeqR2).
+      symmetry in J.
+      apply cmds_rcons2sbs_inv with (sbs:=sbs2)(nbs:=nbs2) in J; auto.
+      destruct J; subst. clear H H6.
+
+      assert (tv_subblocks sbs sbs2 lc1 gl1) as Htv_subblocks'.
         clear - Htv_subblocks.
         admit.
-      apply H0 with (S2:=S2)(Ps2:=Ps2) in Htv_subblocks'; auto.
+      assert (uniq lc1) as Uniqc1. admit.
+      assert (uniq gl1) as Uniqg1. admit.
+      apply H0 with (S2:=S2)(Ps2:=Ps2)(cs2:=cs41) in Htv_subblocks'; auto.
         clear H0.
-        apply dbFdef_func with (l1:=l3)(ps1:=ps3)(sbs1:=sbs3)(tmn1:=tmn2)(la:=la)(lb:=lb2)
-          (lc1:=lc1)(gl1:=gl1)(Mem1:=Mem1)(als1:=als1)(l2:=l2')(ps2:=ps2')(sbs2:=sbs2'); eauto.
-          rewrite <- J1. admit.
 
-        admit. (*uniq*)
-        admit. (*uniq*)
+        apply cmds2nbranchs__nbranchs2cmds in Hcs22nbs1. subst.
+        apply cmds2nbs__nbranchs2cmds in Hcs42nbs2. subst.
+        assert (tv_cmds nbs nbs2 lc2 gl2) as Htv_cmds'.
+          admit. (*tv inclusion*)
+        assert (uniq lc2) as Uniqc2. admit.
+        assert (uniq gl2) as Uniqg2. admit.
+        apply tv_cmds__is__correct with (nbs':=nbs2) in d1; auto.
+          apply dbFdef_func with (l1:=l3)(ps1:=ps3)(cs1:=cs3)(tmn1:=tmn2)(la:=la)(lb:=lb2)
+            (lc1:=lc1)(gl1:=gl1)(Mem1:=Mem1)(als1:=als1)(l2:=l2')(ps2:=ps2')(cs21:=cs41)(cs22:=nbranchs2cmds nbs2)
+            (lc3:=lc3)(als3:=als3)(gl3:=gl3)(Mem3:=Mem3); eauto.
+          admit. (*Wf*) 
         admit. (*Wf*) 
 
       unfold tv_fdef.
       split; auto.
         clear - H5.
         admit. (*tv inclusion*)      
-
-      rewrite <- e0.
-      admit.  (*nth*)
 
 Case "dbFdef_proc".
     rewrite H1 in e. inversion e; subst. clear e.
@@ -437,33 +915,66 @@ Case "dbFdef_proc".
       admit. (*tv inclusion*)      
     apply H with (S2:=S2)(Ps2:=Ps2)(fh1:=fheader_intro rt fid la)(fh2:=fheader_intro rt fid la)(n:=0)
       (ps1':=ps2)(l1':=l2)(als:=nil)(lc':=lc1)(gl':=gl1)
-      (Mem:=Mem0)(Mem':=Mem1)(als':=als1)(tmn1':=insn_return_void rid)(sbs1':=sbs2) 
-      (ps3:=ps1)(sbs3:=sbs1)(tmn2:=tmn1)(l3:=l1)in Htv_blocks; auto.
+      (Mem:=Mem0)(Mem':=Mem1)(als':=als1)(tmn1':=insn_return_void rid)(cs1':=cs21++cs22) 
+      (ps3:=ps1)(cs2:=cs1)(tmn2:=tmn1)(l3:=l1)in Htv_blocks; auto.
       clear H.
-      destruct Htv_blocks as [l3 [ps3 [sbs3 [tmn2 [l2' [ps2' [sbs2' [tmn2' [n' [J1 [J2 [J3 [J4 [J5 J6]]]]]]]]]]]]]].
+      destruct Htv_blocks as [l3 [ps3 [cs3 [tmn2 [l2' [ps2' [cs2' [tmn2' [n' [J1 [J2 [J3 [J4 [J5 J6]]]]]]]]]]]]]].
 
       unfold tv_block in J5.
-      destruct J5 as [EQ [Htv_phinodes [Htv_subblocks EQ']]]; subst.
-      assert (tv_subblocks sbs2 sbs2' lc1 gl1) as Htv_subblocks'.
+
+      remember (cmds2sbs (cs21++cs22)) as R1.
+      remember (cmds2sbs cs2') as R2.
+      destruct R1 as [sbs1 nbs1].
+      destruct R2 as [sbs2 nbs2].
+      destruct J5 as [EQ1 [Htv_phinodes [Htv_subblocks [Htv_cmds EQ2]]]]; subst.
+
+      assert (Hcs21sbs1 := d0).
+      apply dbSubblocks__cmds2sbs in Hcs21sbs1.
+      destruct Hcs21sbs1 as [sbs Hcs21sbs1].
+      assert (Hcs22nbs1 := d1).
+      apply dbCmds2nbranchs in Hcs22nbs1.
+      destruct Hcs22nbs1 as [nbs Hcs22nbs1].
+
+      assert (J:=HeqR1).
+      symmetry in J.
+      apply cmds_rcons2sbs_inv with (sbs:=sbs)(nbs:=nbs) in J; auto using cmds2nbranchs__cmds2nbs.
+      destruct J; subst.
+
+      assert (J:=HeqR2).
+      symmetry in J.
+      apply cmds2sbs_inv in J.
+      destruct J as [cs41 [cs42 [EQ [Hcs41sbs2 Hcs42nbs2]]]]; subst.
+
+      assert (J:=HeqR2).
+      symmetry in J.
+      apply cmds_rcons2sbs_inv with (sbs:=sbs2)(nbs:=nbs2) in J; auto.
+      destruct J; subst. clear H H6.
+
+      assert (tv_subblocks sbs sbs2 lc1 gl1) as Htv_subblocks'.
         clear - Htv_subblocks.
         admit.
-      apply H0 with (S2:=S2)(Ps2:=Ps2) in Htv_subblocks'; auto.
+      assert (uniq lc1) as Uniqc1. admit.
+      assert (uniq gl1) as Uniqg1. admit.
+      apply H0 with (S2:=S2)(Ps2:=Ps2)(cs2:=cs41) in Htv_subblocks'; auto.
         clear H0.
-        apply dbFdef_proc with (l1:=l3)(ps1:=ps3)(sbs1:=sbs3)(tmn1:=tmn2)(la:=la)(lb:=lb2)
-          (lc1:=lc1)(gl1:=gl1)(Mem1:=Mem1)(als1:=als1)(l2:=l2')(ps2:=ps2')(sbs2:=sbs2'); auto.
-          rewrite <- J1. admit.
 
-        admit. (*uniq*)
-        admit. (*uniq*)
+        apply cmds2nbranchs__nbranchs2cmds in Hcs22nbs1. subst.
+        apply cmds2nbs__nbranchs2cmds in Hcs42nbs2. subst.
+        assert (tv_cmds nbs nbs2 lc2 gl2) as Htv_cmds'.
+          admit. (*tv inclusion*)
+        assert (uniq lc2) as Uniqc2. admit.
+        assert (uniq gl2) as Uniqg2. admit.
+        apply tv_cmds__is__correct with (nbs':=nbs2) in d1; auto.
+          apply dbFdef_proc with (l1:=l3)(ps1:=ps3)(cs1:=cs3)(tmn1:=tmn2)(la:=la)(lb:=lb2)
+            (lc1:=lc1)(gl1:=gl1)(Mem1:=Mem1)(als1:=als1)(l2:=l2')(ps2:=ps2')(cs21:=cs41)(cs22:=nbranchs2cmds nbs2)
+            (lc3:=lc3)(als3:=als3)(gl3:=gl3)(Mem3:=Mem3); eauto.
+          admit. (*Wf*) 
         admit. (*Wf*) 
 
       unfold tv_fdef.
       split; auto.
         clear - H5.
         admit. (*tv inclusion*)      
-
-      rewrite <- e0.
-      admit. (*nth*)
 Qed.   
 
 Lemma tv_dbCall__is__correct : forall S1 TD Ps1 lc gl Mem0 call0 lc' gl' Mem' tr S2 Ps2,
@@ -478,15 +989,17 @@ Proof.
   eapply J; eauto.
 Qed.
 
-Definition tv_subblock__is__correct : forall S1 TD Ps1 lc als gl Mem sb1 lc' als' gl' Mem' tr S2 Ps2 sb2,
-  dbSubblock S1 TD Ps1 lc als gl Mem sb1 lc' als' gl' Mem' tr ->
+Definition tv_subblock__is__correct : forall S1 TD Ps1 lc als gl Mem cs1 lc' als' gl' Mem' tr S2 Ps2 cs2 sb1 sb2,
+  dbSubblock S1 TD Ps1 lc als gl Mem cs1 lc' als' gl' Mem' tr ->
   uniq gl ->
   uniq lc ->
+  cmds2sbs cs1 = (sb1::nil, nil) ->
+  cmds2sbs cs2 = (sb2::nil, nil) ->
   wf_subblock sb2 ->
   tv_system S1 S2 ->
   tv_products Ps1 Ps2 ->
   tv_subblock sb1 sb2 lc gl ->
-  dbSubblock S2 TD Ps2 lc als gl Mem sb2 lc' als' gl' Mem' tr.
+  dbSubblock S2 TD Ps2 lc als gl Mem cs2 lc' als' gl' Mem' tr.
 Proof.
   intros.
   destruct tv__is__correct as [_ [J _]].
@@ -494,15 +1007,17 @@ Proof.
   eapply J; eauto.
 Qed.
 
-Lemma tv_subblocks__is__correct : forall S1 TD Ps1 lc als gl Mem sbs1 lc' als' gl' Mem' tr S2 Ps2 sbs2,
-  dbSubblocks S1 TD Ps1 lc als gl Mem sbs1 lc' als' gl' Mem' tr ->
+Lemma tv_subblocks__is__correct : forall S1 TD Ps1 lc als gl Mem cs1 lc' als' gl' Mem' tr S2 Ps2 sbs1 sbs2 cs2,
+  dbSubblocks S1 TD Ps1 lc als gl Mem cs1 lc' als' gl' Mem' tr ->
   uniq gl ->
   uniq lc ->
+  cmds2sbs cs1 = (sbs1, nil) ->
+  cmds2sbs cs2 = (sbs2, nil) ->
   wf_subblocks sbs2 ->
   tv_system S1 S2 ->
   tv_products Ps1 Ps2 ->
   tv_subblocks sbs1 sbs2 lc gl ->
-  dbSubblocks S2 TD Ps2 lc als gl Mem sbs2 lc' als' gl' Mem' tr.
+  dbSubblocks S2 TD Ps2 lc als gl Mem cs2 lc' als' gl' Mem' tr.
 Proof.
   intros.
   destruct tv__is__correct as [_ [_ [J _]]].
